tla-tree/Disk.dfy
@@ -1,0 +1,57 @@
+module Disk {
+
+type Sector(!new,==)
+
+type LBA = int
+datatype Constants = Constants(size:LBA)
+datatype Variables = Variables(sectors:seq<Sector>)
+
+predicate ValidLBA(k:Constants, lba:LBA)
+{
+    0 <= lba < k.size
+}
+
+predicate WF(k:Constants, s:Variables)
+{
+    // All valid lbas are present in the sectors sequence.
+    |s.sectors| == k.size
+}
+
+predicate Init(k:Constants, s:Variables)
+{
+    && WF(k, s)
+}
+
+predicate Peek(k:Constants, s:Variables, lba:LBA, sector:Sector)
+{
+    && WF(k, s)
+    && ValidLBA(k, lba)
+    && s.sectors[lba] == sector
+}
+
+function PeekF(k:Constants, s:Variables, lba:LBA) : Sector
+    requires WF(k, s)
+    requires ValidLBA(k, lba)
+{
+    s.sectors[lba]
+}
+
+predicate Read(k:Constants, s:Variables, s':Variables, lba:LBA, sector:Sector)
+{
+    && Peek(k, s, lba, sector)
+    && s' == s
+}
+
+predicate Write(k:Constants, s:Variables, s':Variables, lba:LBA, sector:Sector)
+{
+    && WF(k, s)
+    && ValidLBA(k, lba)
+    && s'.sectors == s.sectors[lba := sector]
+}
+
+predicate Idle(k:Constants, s:Variables, s':Variables)
+{
+    && s' == s
+}
+
+} // module Disk
