tla-tree/KVTypes.dfy
@@ -1,0 +1,9 @@
+module KVTypes {
+
+type Key(!new,==)
+type Value(!new,==)
+datatype Datum = Datum(key:Key, value:Value)
+
+function EmptyValue() : Value
+
+}
