tla-tree/build.sh
@@ -1,0 +1,7 @@
+#!/bin/bash
+dafny KVTypes.dfy
+dafny Disk.dfy
+dafny CrashableMap.dfy
+dafny CrashSafeLog.dfy
+dafny CrashSafeLogInv.dfy
+dafny CrashSafeLogRefinement.dfy
